nown.v
@@ -17,67 +17,19 @@ Notation iProp := (iProp Σ).
 
 Implicit Types γ : gname.
 
-Definition nown_token γ E : iProp :=
-  gmeta_token γ E.
-
-Lemma nown_token_alloc : ⊢ |==> ∃ γ, nown_token γ ⊤.
-Proof. exact: gmeta_token_alloc. Qed.
-
-Definition nown_ptr γ N γ' : iProp :=
-  gmeta γ N γ'.
-
-#[global]
-Instance nown_ptr_timeless γ N γ' : Timeless (nown_ptr γ N γ').
-Proof. apply _. Qed.
-
-#[global]
-Instance nown_ptr_persistent γ N γ' : Persistent (nown_ptr γ N γ').
-Proof. apply _. Qed.
-
-Lemma nown_ptr_set γ E N γ' :
-  ↑N ⊆ E →
-  nown_token γ E ==∗ nown_ptr γ N γ'.
-Proof. exact: gmeta_set. Qed.
-
-Lemma nown_ptr_agree γ N γ1 γ2 :
-  nown_ptr γ N γ1 -∗
-  nown_ptr γ N γ2 -∗
-  ⌜γ1 = γ2⌝.
-Proof. exact: gmeta_agree. Qed.
-
-Lemma nown_token_difference E1 E2 γ :
-  E1 ⊆ E2 →
-  nown_token γ E2 ⊣⊢ nown_token γ E1 ∗ nown_token γ (E2 ∖ E1).
-Proof.
-move=> ?.
-by rewrite /nown_token -own_op -reservation_map_token_difference.
-Qed.
-
-Arguments nown_token_difference E1 E2 γ : clear implicits.
-
-Lemma nown_token_drop E1 E2 γ :
-  E1 ⊆ E2 →
-  nown_token γ E2 -∗
-  nown_token γ E1.
-Proof.
-iIntros (sub) "t".
-rewrite nown_token_difference //.
-by iDestruct "t" as "[t _]".
-Qed.
-
 Section NOwnLaws.
 
 Context `{!inG Σ A}.
 
 Definition nown γ N (a : A) : iProp :=
-  ∃ γ', nown_ptr γ N γ' ∧ own γ' a.
+  ∃ γ', gmeta γ N γ' ∧ own γ' a.
 
 Lemma nown_alloc γ N E (a : A) :
-  ↑N ⊆ E → ✓ a → nown_token γ E ==∗ nown γ N a ∗ nown_token γ (E ∖ ↑N).
+  ↑N ⊆ E → ✓ a → gmeta_token γ E ==∗ nown γ N a ∗ gmeta_token γ (E ∖ ↑N).
 Proof.
 intros sub valid_a. iIntros "token".
 iMod (own_alloc a) as "(%γ' & own)"; auto.
-rewrite (nown_token_difference (↑N)) //.
+rewrite (gmeta_token_difference (↑N)) //.
 iDestruct "token" as "[tok1 tok2]". iFrame. iExists γ'. iFrame.
 by iApply (gmeta_set with "tok1").
 Qed.
@@ -91,7 +43,7 @@ Lemma nown_valid_2 γ N (a1 a2 : A) :
   nown γ N a1 -∗ nown γ N a2 -∗ ✓ (a1 ⋅ a2).
 Proof.
 iIntros "(%γ1 & #own_γ1 & own1) (%γ2 & #own_γ2 & own2)".
-iPoseProof (nown_ptr_agree with "own_γ1 own_γ2") as "<-".
+iPoseProof (gmeta_agree with "own_γ1 own_γ2") as "<-".
 by iApply (own_valid_2 with "own1 own2").
 Qed.
 
@@ -128,7 +80,7 @@ iSplit.
 - iIntros "(%γ' & #? & [own1 own2])".
   by iSplitL "own1"; iExists γ'; iSplit.
 - iIntros "[(%γ1 & #own_γ1 & own1) (%γ2 & #own_γ2 & own2)]".
-  iPoseProof (nown_ptr_agree with "own_γ1 own_γ2") as "<-".
+  iPoseProof (gmeta_agree with "own_γ1 own_γ2") as "<-".
   iExists γ1. iSplit => //. by iSplitL "own1".
 Qed.
 
@@ -168,6 +120,5 @@ End NOwnLaws.
 
 End NOwn.
 
-#[global] Typeclasses Opaque nown nown_token.
+#[global] Typeclasses Opaque nown.
 Arguments nown_alloc {Σ _ A _ γ} N {_} a.
-Arguments nown_token_difference {Σ _} E1 E2 γ.
