gmeta.v
@@ -9,19 +9,14 @@ Set Implicit Arguments.
 Unset Strict Implicit.
 Unset Printing Implicit Defensive.
 
-Definition metaR := agreeR positiveO.
-
 Class metaGS Σ := {
   metaG_map  : inG Σ (reservation_mapR (agreeR positiveO));
-  metaG_meta : inG Σ metaR;
 }.
 
 Local Existing Instance metaG_map.
-Global Existing Instance metaG_meta.
 
 Definition metaΣ := #[
-  GFunctor (reservation_mapR (agreeR positiveO));
-  GFunctor metaR
+  GFunctor (reservation_mapR (agreeR positiveO))
 ].
 
 Global Instance subG_metaGS Σ : subG metaΣ Σ → metaGS Σ.
@@ -32,27 +27,6 @@ Section Laws.
 Implicit Types (N : namespace) (γ : gname) (E : coPset).
 
 Context `{!metaGS Σ}.
-
-Definition metadata `{Countable L} (x : L) : metaR :=
-  to_agree (encode x).
-
-Lemma metadata_valid `{Countable L} (x : L) : ✓ metadata x.
-Proof. rewrite /metadata. by []. Qed.
-Hint Resolve metadata_valid : core.
-
-#[global]
-Instance metadata_discrete : CmraDiscrete metaR.
-Proof. apply _. Qed.
-
-#[global]
-Instance metadata_core_id `{Countable L} (x : L) : CoreId (metadata x).
-Proof. apply _. Qed.
-
-Lemma metadata_op_inv `{Countable L} (x y : L) :
-  ✓ (metadata x ⋅ metadata y) → x = y.
-Proof.
-by move/to_agree_op_inv/leibniz_equiv_iff/(@encode_inj _ _ _ _ _).
-Qed.
 
 Definition gmeta `{Countable L} γ N (x : L) :=
   own γ (namespace_map_data N (to_agree (encode x))).
@@ -114,8 +88,29 @@ rewrite /gmeta_token -own_op => sub.
 by rewrite -reservation_map_token_difference.
 Qed.
 
+Lemma gmeta_set' `{Countable L} E γ N (x : L) :
+  ↑N ⊆ E →
+  gmeta_token γ E ==∗
+  gmeta γ N x ∗ gmeta_token γ (E ∖ ↑N).
+Proof.
+intros sub. iIntros "token".
+rewrite (@gmeta_token_difference _ (↑N)) //.
+iDestruct "token" as "[tok1 tok2]". iFrame.
+by iApply (gmeta_set with "tok1").
+Qed.
+
+Lemma gmeta_token_drop E1 E2 γ :
+  E1 ⊆ E2 →
+  gmeta_token γ E2 -∗
+  gmeta_token γ E1.
+Proof.
+iIntros (sub) "t".
+rewrite gmeta_token_difference //.
+by iDestruct "t" as "[t _]".
+Qed.
+
 End Laws.
 
 Arguments gmeta_token_difference {Σ _} γ E1 E2.
 Arguments gmeta_set {Σ _ _ _ _} E γ N x.
-Global Typeclasses Opaque metadata metaR.
+Arguments gmeta_set' {Σ _ _ _ _} E γ N x.
